test/oneoff/specialization_plan/ExternSemanticStrength.v
@@ -55,3 +55,52 @@ Proof.
     as [represented_args [extern_outcome [call_representation _]]].
   exact call_representation.
 Qed.
+
+Definition extern_observation
+    (extern_execution outcomes_refine : Prop) : Semantics :=
+  {| sem_value := unit;
+     sem_outcome := unit;
+     sem_arguments_well_typed := fun _ _ => True;
+     sem_represented_values_valid := fun _ _ => True;
+     sem_value_well_typed := fun _ _ => True;
+     sem_represented_value_valid := fun _ _ => True;
+     sem_value_satisfies_bound := fun _ _ => True;
+     sem_arguments_represent := fun _ _ _ _ => True;
+     sem_represents := fun _ _ _ _ => True;
+     sem_sail_eval := fun _ _ _ => True;
+     sem_jib_eval := fun _ _ _ => True;
+     sem_conversion_eval := fun _ _ _ _ _ => True;
+     sem_call_arguments_represent := fun _ _ _ => True;
+     sem_sail_call := fun _ _ _ _ => True;
+     sem_jib_call := fun _ _ _ _ _ => True;
+     sem_extern_eval := fun _ _ _ => extern_execution;
+     sem_sail_reachable := fun _ _ => True;
+     sem_bounds_hold := fun _ _ => True;
+     sem_outcomes_refine := fun _ _ => outcomes_refine;
+     sem_exceptions_equivalent := fun _ _ => True;
+     sem_lifetime_compatible := fun _ _ _ => True |}.
+
+Definition missing_extern_execution : Semantics :=
+  extern_observation False True.
+
+Theorem extern_requires_extern_execution :
+  ~ obligation_4e81ef1ad207ac8ec4288e2a2826812a missing_extern_execution.
+Proof.
+  intro obligation.
+  destruct (obligation [] tt I)
+    as [represented_args [extern_outcome [_ [extern_execution _]]]].
+  exact extern_execution.
+Qed.
+
+Definition missing_extern_outcome_refinement : Semantics :=
+  extern_observation True False.
+
+Theorem extern_requires_outcome_refinement :
+  ~ obligation_4e81ef1ad207ac8ec4288e2a2826812a
+      missing_extern_outcome_refinement.
+Proof.
+  intro obligation.
+  destruct (obligation [] tt I)
+    as [represented_args [extern_outcome [_ [_ refinement]]]].
+  exact refinement.
+Qed.
